name store-safe evidence-at prefix route

rocq/theories/TypeSystem/TypeSafetyDirectCallRoute.v
@@ -302,6 +302,31 @@ Definition eval_preserves_typing_roots_synthetic_direct_call_ready_summary_at_pr
       store_no_shadow s' /\
       root_env_no_shadow R'.
 
+Definition eval_preserves_typing_roots_store_safe_synthetic_direct_call_ready_summary_at_prefix_call_statement_evidence_at
+    : Prop :=
+  forall env s fname args s' v,
+    eval env s (ECall fname args) s' v ->
+    forall (Ω : outlives_ctx) (n : nat) R Σ T Σ' R' roots,
+      store_safe_function_value_call_args env args ->
+      store_typed_prefix env s Σ ->
+      store_roots_within R s ->
+      store_no_shadow s ->
+      root_env_no_shadow R ->
+      root_env_store_roots_named R s ->
+      root_env_store_keys_named R s ->
+      typed_env_roots env Ω n R Σ (ECall fname args) T Σ' R' roots ->
+      fn_env_unique_by_name env ->
+      fn_root_shadow_synthetic_direct_call_ready_summary_evidence_at env fname ->
+      direct_call_callee_body_root_synthetic_direct_call_ready_evidence_at
+        env fname ->
+      store_typed_prefix env s' Σ' /\
+      value_has_type env s' v T /\
+      store_ref_targets_preserved env s s' /\
+      store_roots_within R' s' /\
+      value_roots_within roots v /\
+      store_no_shadow s' /\
+      root_env_no_shadow R'.
+
 Lemma direct_call_callee_body_root_synthetic_direct_call_ready_evidence_of_evidence_at_all :
   forall env,
     (forall fname,
@@ -7154,6 +7179,94 @@ Proof.
   - rewrite Hremoved_exact. exact Hroots_args.
   - eapply direct_call_value_roots_within_store_subset; eassumption.
   - rewrite Hremoved_exact. exact Hshadow_args.
+Qed.
+
+
+Theorem eval_preserves_typing_roots_store_safe_synthetic_direct_call_ready_summary_at_prefix_call_statement_evidence_at_of_body_call_callback :
+  eval_preserves_frame_param_scope_synthetic_direct_call_ready_statement ->
+  eval_preserves_typing_ready_prefix_mutual_statement ->
+  eval_preserves_typing_roots_ready_prefix_mutual_statement ->
+  eval_preserves_roots_ready_mutual_statement ->
+  eval_preserves_root_names_ready_mutual_statement ->
+  eval_preserves_root_keys_named_ready_mutual_statement ->
+  (forall env fname fdef fcall used used' fname_body args_body synthetic_body,
+    In fdef (env_fns env) ->
+    fn_name fdef = fname ->
+    alpha_rename_fn_def used fdef = (fcall, used') ->
+    direct_call_target_expr (fn_body fcall) =
+      Some (fname_body, args_body, synthetic_body) ->
+    fn_root_shadow_synthetic_direct_call_ready_summary_evidence_at
+      (global_env_with_local_bounds env (fn_bounds fcall)) fname_body) ->
+  (forall env fname fdef fcall used used' s_args s_body vs ret R_args arg_roots
+      fname_body args_body T_body Gamma_out R_body roots_body,
+    In fdef (env_fns env) ->
+    fn_name fdef = fname ->
+    alpha_rename_fn_def used fdef = (fcall, used') ->
+    direct_call_target_expr (fn_body fcall) =
+      Some (fname_body, args_body, ECall fname_body args_body) ->
+    preservation_ready_args args_body ->
+    typed_env_roots (global_env_with_local_bounds env (fn_bounds fcall))
+      (fn_outlives fcall) (fn_lifetimes fcall)
+      (call_param_root_env (fn_params fcall) arg_roots R_args)
+      (sctx_of_ctx (params_ctx (fn_params fcall)))
+      (ECall fname_body args_body) T_body (sctx_of_ctx Gamma_out) R_body
+      roots_body ->
+    fn_env_unique_by_name (global_env_with_local_bounds env (fn_bounds fcall)) ->
+    fn_root_shadow_synthetic_direct_call_ready_summary_evidence_at
+      (global_env_with_local_bounds env (fn_bounds fcall)) fname_body ->
+    direct_call_callee_body_root_synthetic_direct_call_ready_evidence_at
+      (global_env_with_local_bounds env (fn_bounds fcall)) fname_body ->
+    store_typed_prefix (global_env_with_local_bounds env (fn_bounds fcall))
+      (bind_params (fn_params fcall) vs s_args)
+      (sctx_of_ctx (params_ctx (fn_params fcall))) ->
+    store_roots_within
+      (call_param_root_env (fn_params fcall) arg_roots R_args)
+      (bind_params (fn_params fcall) vs s_args) ->
+    store_no_shadow (bind_params (fn_params fcall) vs s_args) ->
+    root_env_no_shadow
+      (call_param_root_env (fn_params fcall) arg_roots R_args) ->
+    root_env_store_roots_named
+      (call_param_root_env (fn_params fcall) arg_roots R_args)
+      (bind_params (fn_params fcall) vs s_args) ->
+    root_env_store_keys_named
+      (call_param_root_env (fn_params fcall) arg_roots R_args)
+      (bind_params (fn_params fcall) vs s_args) ->
+    eval (global_env_with_local_bounds env (fn_bounds fcall))
+      (bind_params (fn_params fcall) vs s_args)
+      (ECall fname_body args_body) s_body ret ->
+    store_typed_prefix (global_env_with_local_bounds env (fn_bounds fcall))
+      s_body (sctx_of_ctx Gamma_out) /\
+    value_has_type (global_env_with_local_bounds env (fn_bounds fcall))
+      s_body ret T_body /\
+    store_ref_targets_preserved
+      (global_env_with_local_bounds env (fn_bounds fcall))
+      (bind_params (fn_params fcall) vs s_args) s_body /\
+    store_roots_within R_body s_body /\
+    value_roots_within roots_body ret /\
+    store_no_shadow s_body /\
+    root_env_no_shadow R_body) ->
+  eval_preserves_typing_roots_store_safe_synthetic_direct_call_ready_summary_at_prefix_call_statement_evidence_at.
+Proof.
+  intros Hscope_synthetic Htyping_prefix Hprefix_ready Hroots_ready Hroot_names
+    Hroot_keys Hsummary_body_at_all Hbody_call_callback_all env s fname args s'
+    v Heval Omega n R Sigma T Sigma' R' roots Hsafe_args Hstore Hroots
+    Hshadow Hrn Hnamed Hkeys Htyped Hunique Hsummary_at Hevidence_at.
+  destruct
+    (eval_preserves_typing_roots_store_safe_synthetic_direct_call_ready_ecall_cleanup_bridge_with_alpha_evidence_at_body_call_callback_prefix_store_final_roots_core
+      Hscope_synthetic Htyping_prefix Hprefix_ready Hroots_ready Hroot_names
+      Hroot_keys env s s' v fname args Heval Omega n R Sigma T Sigma'
+      R' roots Hsafe_args Hstore Hroots Hshadow Hrn Hnamed Hkeys Htyped
+      Hunique Hsummary_at
+      (fun fdef fcall used used' fname_body args_body synthetic_body =>
+        Hsummary_body_at_all env fname fdef fcall used used' fname_body
+          args_body synthetic_body)
+      (fun fdef fcall used used' s_args s_body vs ret R_args arg_roots
+          fname_body args_body T_body Gamma_out R_body roots_body =>
+        Hbody_call_callback_all env fname fdef fcall used used' s_args
+          s_body vs ret R_args arg_roots fname_body args_body T_body
+          Gamma_out R_body roots_body))
+    as [Hstore' [Hv [Hpres [Hroots' [Hvroots [Hshadow' Hrn']]]]]].
+  repeat split; try assumption.
 Qed.
 
 
